Instances/BoolType/Boolean.v
@@ -1,0 +1,18 @@
+Require Import Classes.BoolType.
+Require Import Language.Statements.
+Require Import Types.State.
+Require Import Types.AbstractStore.
+Require Import Types.Result.
+
+Definition ensure_bool (v : cvalue) : State bool :=
+  fun st => match v with
+            | VBool b => returnR bool store b st
+            | _ => crashed _ _
+            end.
+  
+Instance boolean_type : BoolType bool :=
+{
+  ensure_boolean := ensure_bool;
+  and_op := andb;
+  neg_op := negb;
+}.
