Classes/BoolType.v
@@ -1,0 +1,10 @@
+Class BoolType 
+  {V : Type}
+  {state : Type -> Type }
+  (B : Type)
+  : Type :=
+{
+  ensure_boolean : V -> state B;
+  and_op : B -> B -> B;
+  neg_op : B -> B;
+}.
